SKAT, Boolean algebra stuff, fixed KAT, shifted KA tactic

Carrier/Dioid.thy
@@ -2,6 +2,10 @@ theory Dioid
   imports Lattice
 begin
 
+(* +------------------------------------------------------------------------+ *)
+subsection {* Dioids *}
+(* +------------------------------------------------------------------------+ *)
+
 record 'a dioid = "'a partial_object" +
   plus :: "'a \<Rightarrow> 'a \<Rightarrow> 'a" (infixl "+\<index>" 70)
   mult :: "'a \<Rightarrow> 'a \<Rightarrow> 'a" (infixl "\<cdot>\<index>" 80)
@@ -79,5 +83,143 @@ begin
     and nat_trans = order_trans[simplified]
 
 end
+
+(* +------------------------------------------------------------------------+ *)
+subsection {* Free Dioid *}
+(* +------------------------------------------------------------------------+ *)
+
+datatype 'a dioid_term = DioidAtom 'a
+                       | DioidPlus "'a dioid_term" "'a dioid_term"
+                       | DioidMult "'a dioid_term" "'a dioid_term"
+                       | DioidOne
+                       | DioidZero
+
+primrec (in dioid) term_unfold :: "'a dioid_term \<Rightarrow> 'a" where
+  "term_unfold (DioidAtom x) = x"
+| "term_unfold (DioidPlus x y) = (term_unfold x) + (term_unfold y)"
+| "term_unfold (DioidMult x y) = (term_unfold x) \<cdot> (term_unfold y)"
+| "term_unfold DioidOne = 1"
+| "term_unfold DioidZero = 0"
+
+lemma (in dioid) term_fold_atom: "x \<in> carrier A \<Longrightarrow> x = term_unfold (DioidAtom x)"
+  by (rule term_unfold.simps(1)[symmetric])
+
+primrec (in dioid) term_atoms :: "'a dioid_term \<Rightarrow> 'a set" where
+  "term_atoms (DioidAtom x) = {x}"
+| "term_atoms (DioidPlus x y) = (term_atoms x) \<union> (term_atoms y)"
+| "term_atoms (DioidMult x y) = (term_atoms x) \<union> (term_atoms y)"
+| "term_atoms DioidOne = {}"
+| "term_atoms DioidZero = {}"
+
+lemma (in dioid) term_closure: "term_atoms x \<subseteq> carrier A \<Longrightarrow> term_unfold x \<in> carrier A"
+  by (induct x, simp_all add: add_closed mult_closed one_closed zero_closed)
+
+primrec dioid_term_map :: "('a \<Rightarrow> 'b) \<Rightarrow> 'a dioid_term \<Rightarrow> 'b dioid_term" where
+  "dioid_term_map f (DioidAtom x) = DioidAtom (f x)"
+| "dioid_term_map f (DioidPlus x y) = DioidPlus (dioid_term_map f x) (dioid_term_map f y)"
+| "dioid_term_map f (DioidMult x y) = DioidMult (dioid_term_map f x) (dioid_term_map f y)"
+| "dioid_term_map f DioidOne = DioidOne"
+| "dioid_term_map f DioidZero = DioidZero"
+
+inductive dioid_con :: "'a dioid_term \<Rightarrow> 'a dioid_term \<Rightarrow> bool" where
+  refl [intro]: "dioid_con x x"
+| sym [sym]: "dioid_con x y \<Longrightarrow> dioid_con y x"
+| trans [trans]: "dioid_con x y \<Longrightarrow> dioid_con y z \<Longrightarrow> dioid_con x z"
+| add_lift: "dioid_con x1 x2 \<Longrightarrow> dioid_con y1 y2 \<Longrightarrow> dioid_con (DioidPlus x1 y1) (DioidPlus x2 y2)"
+| mult_lift: "dioid_con x1 x2 \<Longrightarrow> dioid_con y1 y2 \<Longrightarrow> dioid_con (DioidMult x1 y1) (DioidMult x2 y2)"
+| mult_assoc: "dioid_con (DioidMult (DioidMult x y) z) (DioidMult x (DioidMult y z))"
+| add_assoc: "dioid_con (DioidPlus (DioidPlus x y) z) (DioidPlus x (DioidPlus y z))"
+| add_comm: "dioid_con (DioidPlus x y) (DioidPlus y x)"
+| add_idem: "dioid_con (DioidPlus x x) x"
+| distl: "dioid_con (DioidMult x (DioidPlus y z)) (DioidPlus (DioidMult x y) (DioidMult x z))"
+| distr: "dioid_con (DioidMult (DioidPlus x y) z) (DioidPlus (DioidMult x z) (DioidMult y z))"
+| mult_onel: "dioid_con (DioidMult DioidOne x) x"
+| mult_oner: "dioid_con (DioidMult x DioidOne) x"
+| add_zerol: "dioid_con (DioidPlus DioidZero x) x"
+| mult_zerol: "dioid_con (DioidMult DioidZero x) DioidZero"
+| mult_zeror: "dioid_con (DioidMult x DioidZero) DioidZero"
+
+quotient_type 'a dioid_expr = "'a dioid_term" / dioid_con
+  by (metis (lifting) dioid_con.refl dioid_con.sym dioid_con.trans equivpI reflpI sympI transpI)
+
+lift_definition term_mult :: "'a dioid_expr \<Rightarrow> 'a dioid_expr \<Rightarrow> 'a dioid_expr" is DioidMult
+  by (rule mult_lift, assumption+)
+
+lift_definition term_plus :: "'a dioid_expr \<Rightarrow> 'a dioid_expr \<Rightarrow> 'a dioid_expr" is DioidPlus
+  by (rule add_lift, assumption+)
+
+lift_definition term_one :: "'a dioid_expr" is DioidOne
+  by (rule dioid_con.refl)
+
+lift_definition term_zero :: "'a dioid_expr" is DioidZero
+  by (rule dioid_con.refl)
+
+definition free_dioid :: "'a dioid_expr dioid" where
+  "free_dioid = \<lparr>carrier = UNIV, plus = term_plus, mult = term_mult, one = term_one, zero = term_zero\<rparr>"
+
+lemma "dioid free_dioid"
+proof (unfold_locales, simp_all add: free_dioid_def)
+  fix x y z
+  show "term_mult (term_mult x y) z = term_mult x (term_mult y z)"
+    by (transfer, rule dioid_con.mult_assoc)
+  show "term_plus (term_plus x y) z = term_plus x (term_plus y z)"
+    by (transfer, rule dioid_con.add_assoc)
+  show "term_plus x y = term_plus y x"
+    by (transfer, rule dioid_con.add_comm)
+  show "term_plus x x = x"
+    by (transfer, rule dioid_con.add_idem)
+  show "term_mult x (term_plus y z) = term_plus (term_mult x y) (term_mult x z)"
+    by (transfer, rule dioid_con.distl)
+  show "term_mult (term_plus x y) z = term_plus (term_mult x z) (term_mult y z)"
+    by (transfer, rule dioid_con.distr)
+  show "term_mult term_one x = x"
+    by (transfer, rule dioid_con.mult_onel)
+  show "term_mult x term_one = x"
+    by (transfer, rule dioid_con.mult_oner)
+  show "term_plus term_zero x = x"
+    by (transfer, rule dioid_con.add_zerol)
+  show "term_mult term_zero x = term_zero"
+    by (transfer, rule dioid_con.mult_zerol)
+  show "term_mult x term_zero = term_zero"
+    by (transfer, rule dioid_con.mult_zeror)
+qed
+
+ML {*
+
+fun term_fold_tac fold_atom folds closure leaves =
+  Subgoal.FOCUS (fn {context, prems, ...} =>
+  let
+    val witnesses = Locale.get_witnesses context
+    val subst_thm = hd (witnesses RL [fold_atom])
+    val subst_thms = prems RL [subst_thm]
+    val folds = witnesses RL folds
+    val to_leaves_thm = hd (witnesses RL [closure])
+  in
+    DETERM
+      (Method.insert_tac subst_thms 1
+      THEN REPEAT (etac @{thm ssubst} 1)
+      THEN asm_full_simp_tac (HOL_basic_ss addsimps folds) 1)
+    THEN (if leaves then rtac to_leaves_thm 1 else all_tac)
+  end)
+
+val dioid_term_fold_tac =
+  term_fold_tac @{thm dioid.term_fold_atom} @{thms dioid.term_unfold.simps[symmetric]} @{thm dioid.term_closure}
+
+*}
+
+method_setup dioid_closure = {*
+Scan.succeed (fn ctxt =>
+  let
+    val witnesses = Locale.get_witnesses ctxt
+    val unfolds = witnesses RL @{thms dioid.term_atoms.simps}
+  in
+    METHOD (fn _ =>
+      dioid_term_fold_tac true ctxt 1
+      THEN asm_full_simp_tac (@{simpset} addsimps unfolds) 1)
+  end)
+*}
+
+lemma (in dioid) "\<lbrakk>y\<cdot>y \<in> carrier A; x \<in> carrier A\<rbrakk> \<Longrightarrow> x + x + y\<cdot>y \<in> carrier A"
+  by dioid_closure
 
 end
