Carrier/Kleene_Algebra.thy
@@ -1,5 +1,5 @@
 theory Kleene_Algebra
-  imports Dioid "Regular-Sets/Equivalence_Checking"
+  imports Dioid
 begin
 
 (* +------------------------------------------------------------------------+ *)
@@ -65,392 +65,155 @@ begin
 
 end
 
-(* +------------------------------------------------------------------------+ *)
-subsection {* Free Kleene Algebra *}
-(* +------------------------------------------------------------------------+ *)
+datatype 'a ka_term = KAAtom 'a
+                    | KAPlus "'a ka_term" "'a ka_term"
+                    | KAMult "'a ka_term" "'a ka_term"
+                    | KAStar "'a ka_term"
+                    | KAOne
+                    | KAZero
 
-inductive_set languages :: "'a set \<Rightarrow> 'a lang" for \<Sigma> :: "'a set" where
-  "[] \<in> languages \<Sigma>"
-| "\<lbrakk>x \<in> \<Sigma>; xs \<in> languages \<Sigma>\<rbrakk> \<Longrightarrow> x#xs \<in> languages \<Sigma>"
+primrec (in kleene_algebra) ka_term_unfold :: "'a ka_term \<Rightarrow> 'a" where
+  "ka_term_unfold (KAAtom x) = x"
+| "ka_term_unfold (KAPlus x y) = (ka_term_unfold x) + (ka_term_unfold y)"
+| "ka_term_unfold (KAMult x y) = (ka_term_unfold x) \<cdot> (ka_term_unfold y)"
+| "ka_term_unfold (KAStar x) = (ka_term_unfold x)\<^sup>\<star>"
+| "ka_term_unfold KAOne = 1"
+| "ka_term_unfold KAZero = 0"
 
-lemma languages_empty [simp]: "languages {} = {[]}"
-  by (metis equals0D insert_iff languages.simps nonempty_iff)
+lemma (in kleene_algebra) ka_term_fold_atom:
+  "x \<in> carrier A \<Longrightarrow> x = ka_term_unfold (KAAtom x)"
+  by (rule ka_term_unfold.simps(1)[symmetric])
 
-inductive_set free_ka_set :: "'a set \<Rightarrow> 'a lang set" for \<Sigma> :: "'a set" where
-  empty: "{} \<in> free_ka_set \<Sigma>"
-| lang: "x \<in> languages \<Sigma> \<Longrightarrow> {x} \<in> free_ka_set \<Sigma>"
-| union: "\<lbrakk>p \<in> free_ka_set \<Sigma>; q \<in> free_ka_set \<Sigma>\<rbrakk> \<Longrightarrow> p \<union> q \<in> free_ka_set \<Sigma>"
-| concat: "\<lbrakk>p \<in> free_ka_set \<Sigma>; q \<in> free_ka_set \<Sigma>\<rbrakk> \<Longrightarrow> p @@ q \<in> free_ka_set \<Sigma>"
-| star: "p \<in> free_ka_set \<Sigma> \<Longrightarrow> Regular_Set.star p \<in> free_ka_set \<Sigma>"
+primrec (in kleene_algebra) ka_term_atoms :: "'a ka_term \<Rightarrow> 'a set" where
+  "ka_term_atoms (KAAtom x) = {x}"
+| "ka_term_atoms (KAPlus x y) = (ka_term_atoms x) \<union> (ka_term_atoms y)"
+| "ka_term_atoms (KAMult x y) = (ka_term_atoms x) \<union> (ka_term_atoms y)"
+| "ka_term_atoms (KAStar x) = ka_term_atoms x"
+| "ka_term_atoms KAOne = {}"
+| "ka_term_atoms KAZero = {}"
 
-lemma free_ka_set_empty [simp]: "free_ka_set {} = {{}, {[]}}"
-proof
-  show "free_ka_set {} \<subseteq> {{}, {[]}}"
-  proof
-    fix x assume "x \<in> free_ka_set {}"
-    thus "x \<in> {{}, {[]}}"
-      apply (induct x)
-      apply simp
-      apply simp
-      apply (metis empty_iff insert_iff sup_bot_left sup_bot_right sup_idem)
-      apply (metis conc_empty(2) conc_epsilon(2) insert_iff singleton_iff)
-      by (metis empty_iff insert_iff star_empty star_insert_eps)
-  qed
-  show "{{}, {[]}} \<subseteq> free_ka_set {}"
-    apply (auto, metis free_ka_set.empty)
-    by (metis free_ka_set.lang languages.intros(1))
-qed
-
-definition free_ka :: "'a set \<Rightarrow> 'a lang kleene_algebra" where
-  "free_ka \<Sigma> \<equiv> \<lparr>carrier = free_ka_set \<Sigma>, plus = op \<union>, mult = op @@, one = {[]}, zero = {}, star = Regular_Set.star\<rparr>"
-
-lemma "carrier \<in> {K. kleene_algebra K} \<rightarrow> UNIV"
-  by (simp add: ftype_def)
-
-lemma free_ka_dioid: "dioid (free_ka \<Sigma>)"
-  apply (default, simp_all add: free_ka_def)
-  apply (metis free_ka_set.union)
-  apply (metis free_ka_set.concat)
-  apply (metis free_ka_set.lang languages.intros(1))
-  apply (metis free_ka_set.empty)
-  apply (metis conc_assoc)
-  by auto
-
-lemma lang_inf_distl:
-  assumes xc: "x \<in> free_ka_set \<Sigma>"
-  and Xc: "X \<subseteq> free_ka_set \<Sigma>"
-  shows "x @@ \<Union> X = \<Union> {x @@ y |y. y \<in> X}"
-  by fast
-
-lemma lang_inf_distr:
-  assumes xc: "x \<in> free_ka_set \<Sigma>"
-  and Xc: "X \<subseteq> free_ka_set \<Sigma>"
-  shows "\<Union> X @@ x = \<Union> {y @@ x |y. y \<in> X}"
-  by fast
-
-lemma RStar_inductr_var:
-  assumes xc: "x \<in> free_ka_set \<Sigma>" and yc: "y \<in> free_ka_set \<Sigma>"
-  and asm: "y @@ x \<subseteq> y" shows "y @@ Regular_Set.star x \<subseteq> y"
-proof -
-  have "\<forall>n. y @@ x ^^ n \<subseteq> y"
-  proof (intro allI)
-    fix n show "y @@ x ^^ n \<subseteq> y"
-      apply (induct n, simp)
-      by (smt Un_absorb1 Un_upper1 asm conc_Un_distrib(2) conc_assoc lang_pow.simps(2) order_trans)
-  qed
-  hence "(\<Union>n. y @@ x ^^ n) \<subseteq> y"
-    by (metis (lifting) SUP_le_iff)
-  thus ?thesis
-    by (metis Regular_Set.star_def conc_UNION_distrib(1))
-qed
-
-lemma RStar_inductr:
-  assumes xc: "x \<in> free_ka_set \<Sigma>"
-  and yc: "y \<in> free_ka_set \<Sigma>"
-  and zc: "z \<in> free_ka_set \<Sigma>"
-  shows "z \<union> y @@ x \<subseteq> y \<longrightarrow> z @@ Regular_Set.star x \<subseteq> y"
-proof
-  assume hyp: "z \<union> y @@ x \<subseteq> y"
-  hence "z \<subseteq> y" and "y @@ x \<subseteq> y"
-    by blast+
-  hence "y @@ Regular_Set.star x \<subseteq> y"
-    by (metis RStar_inductr_var xc yc)
-  thus "z @@ Regular_Set.star x \<subseteq> y"
-    using `z \<subseteq> y` by blast
-qed
-
-lemma RStar_inductl_var:
-  assumes xc: "x \<in> free_ka_set \<Sigma>" and yc: "y \<in> free_ka_set \<Sigma>"
-  and asm: "x @@ y \<subseteq> y" shows "Regular_Set.star x @@ y \<subseteq> y"
-proof -
-  have "\<forall>n. x ^^ n @@ y \<subseteq> y"
-  proof (intro allI)
-    fix n show "x ^^ n @@ y \<subseteq> y"
-      apply (induct n, simp)
-      by (smt asm conc_Un_distrib(1) conc_assoc lang_pow.simps(2) lang_pow_code_def order_trans subset_Un_eq)
-  qed
-  hence "(\<Union>n. x ^^ n @@ y) \<subseteq> y"
-    by (metis (lifting) SUP_le_iff)
-  thus ?thesis
-    by (metis Regular_Set.star_def conc_UNION_distrib(2))
-qed
-
-lemma RStar_inductl:
-  assumes xc: "x \<in> free_ka_set \<Sigma>"
-  and yc: "y \<in> free_ka_set \<Sigma>"
-  and zc: "z \<in> free_ka_set \<Sigma>"
-  shows "z \<union> x @@ y \<subseteq> y \<longrightarrow> Regular_Set.star x @@ z \<subseteq> y"
-proof
-  assume hyp: "z \<union> x @@ y \<subseteq> y"
-  hence "z \<subseteq> y" and "x @@ y \<subseteq> y"
-    by blast+
-  hence "Regular_Set.star x @@ y \<subseteq> y"
-    by (metis RStar_inductl_var xc yc)
-  thus "Regular_Set.star x @@ z \<subseteq> y"
-    using `z \<subseteq> y` by blast
-qed
-
-lemma free_ka_prop:
-  shows "kleene_algebra (free_ka \<Sigma>)"
-  apply (simp add: kleene_algebra_def kleene_algebra_axioms_def, safe)
-  apply (rule free_ka_dioid)
-  apply (simp_all add: dioid.nat_order_def[OF free_ka_dioid])
-  apply (simp_all add: free_ka_def)
-  apply (rule free_ka_set.star, assumption)
-  apply (metis (lifting) Un_insert_left Un_insert_right star_unfold_left sup_left_idem)
-  apply (metis (lifting) Un_insert_left Un_insert_right conc_star_comm star_unfold_left sup.idem sup.left_idem)
-  apply (metis RStar_inductl inf_sup_ord(4) sup_absorb1 sup_commute)
-  by (metis (lifting) RStar_inductr subset_Un_eq)
-
-(* +------------------------------------------------------------------------+ *)
-subsection {* Decision Procedure for KA *}
-(* +------------------------------------------------------------------------+ *)
-
-lemma atoms_finite: "finite (atoms x)"
-  by (induct x, simp_all)
-
-lemma rexp_in_fka:
-  shows "lang x \<in> free_ka_set (atoms x \<union> y)"
-  apply (induct x arbitrary: y, simp_all)
-  apply (metis free_ka_set.empty)
-  apply (metis free_ka_set.lang languages.intros(1))
-  apply (metis free_ka_set.lang insertI1 languages.intros(1) languages.intros(2))
-  apply (metis free_ka_set.union sup_commute sup_left_commute)
-  apply (metis (lifting) Un_assoc Un_left_commute free_ka_set.concat)
-  by (metis free_ka_set.star)
-
-lemma fka_lang: "x \<in> free_ka_set \<Sigma> \<Longrightarrow> \<exists>y. lang y = x"
-proof (induct x rule: free_ka_set.induct)
-  show "\<exists>y. lang y = {}"
-    by (rule_tac x = Zero in exI, simp)
-next
-  fix z assume "z \<in> languages \<Sigma>"
-  thus "\<exists>y. lang y = {z}"
-  proof (induct z)
-    show "\<exists>y. lang y = {[]}"
-      by (rule_tac x = "One" in exI, simp)
-    fix x xs assume "\<exists>y. lang y = {xs}"
-    then obtain y where "lang y = {xs}" by auto
-    thus "\<exists>y. lang y = {x # xs}"
-      by (rule_tac x = "Times (Atom x) y" in exI, simp add: conc_def)
-  qed
-next
-  fix p q assume "p \<in> free_ka_set \<Sigma>" "\<exists>y. lang y = p"
-  and "q \<in> free_ka_set \<Sigma>" "\<exists>y. lang y = q"
-  then obtain y1 y2 where "lang y1 = p" and "lang y2 = q" by auto
-  thus "\<exists>y. lang y = p \<union> q"
-    by (rule_tac x = "Plus y1 y2" in exI, simp)
-next
-  fix p q assume "p \<in> free_ka_set \<Sigma>" "\<exists>y. lang y = p"
-  and "q \<in> free_ka_set \<Sigma>" "\<exists>y. lang y = q"
-  then obtain y1 y2 where "lang y1 = p" and "lang y2 = q" by auto
-  thus "\<exists>y. lang y = conc p q"
-    by (rule_tac x = "Times y1 y2" in exI, simp)
-next
-  fix p assume "p \<in> free_ka_set \<Sigma>" "\<exists>y. lang y = p"
-  then obtain y where "lang y = p" by auto
-  thus "\<exists>y. lang y = Regular_Set.star p"
-    by (rule_tac x = "Star y" in exI, simp)
-qed
-
-fun change_atoms :: "('a \<Rightarrow> 'b) \<Rightarrow> 'a rexp \<Rightarrow> 'b rexp" where
-  "change_atoms f (Atom x) = Atom (f x)"
-| "change_atoms f (Plus x y) = Plus (change_atoms f x) (change_atoms f y)"
-| "change_atoms f (Times x y) = Times (change_atoms f x) (change_atoms f y)"
-| "change_atoms f One = One"
-| "change_atoms f Zero = Zero"
-| "change_atoms f (Star x) = Star (change_atoms f x)"
-
-lemma change_atoms_inv:
-  assumes surjf: "surj f"
-  shows "change_atoms f (change_atoms (inv f) x) = x"
-  by (induct x, simp_all, metis assms surj_iff_all)
-
-lemma change_atoms_surj:
-  assumes surjf: "surj f"
-  shows "surj (change_atoms f)"
-  by (metis assms change_atoms_inv surjI)
-
-definition lang_map :: "('a \<Rightarrow> 'b) \<Rightarrow> 'a lang \<Rightarrow> 'b lang" where
-  "lang_map f x \<equiv> map f ` x"
-
-lemma lang_map_def_var: "lang_map f = (\<lambda>x. map f ` x)"
-  by (default, simp add: lang_map_def)
-
-lemma bij_map: "bij f \<Longrightarrow> bij (map f)"
-  by (simp add: bij_def surj_def, metis ex_map_conv)
-
-lemma bij_image: "bij f \<Longrightarrow> bij (op ` f)"
-  apply (auto simp add: bij_def surj_def inj_on_def image_def)
-  apply blast
-  apply blast
-  apply (rule_tac x = "inv f ` x" in exI)
-  apply (subgoal_tac "\<And>a. f (inv f a) = a")
-  apply simp
-  by (smt CollectD UNIV_I inv_def tfl_some)
-
-lemma bij_lang_map: "bij f \<Longrightarrow> bij (lang_map f)"
-  by (simp add: lang_map_def_var, metis bij_image bij_map)
-
-lemma image_conc: "map f ` (\<alpha> @@ \<beta>) = map f ` \<alpha> @@ map f ` \<beta>"
-proof (simp add: conc_def)
-  have "map f ` {xs @ ys |xs ys. xs \<in> \<alpha> \<and> ys \<in> \<beta>} = {map f (xs @ ys) |xs ys. xs \<in> \<alpha> \<and> ys \<in> \<beta>}"
-    by blast
-  also have "... = {(map f xs @ map f ys) |xs ys. xs \<in> \<alpha> \<and> ys \<in> \<beta>}"
-    by (smt Collect_cong map_append)
-  also have "... = {(xs @ ys) |xs ys. xs \<in> map f ` \<alpha> \<and> ys \<in> map f ` \<beta>}"
-    by blast
-  finally show "map f ` {xs @ ys |xs ys. xs \<in> \<alpha> \<and> ys \<in> \<beta>} = {xs @ ys |xs ys. xs \<in> map f ` \<alpha> \<and> ys \<in> map f ` \<beta>}" .
-qed
-
-lemma image_star1: "map f ` Regular_Set.star x \<subseteq> Regular_Set.star (map f ` x)"
-proof auto
-  fix a assume "a \<in> Regular_Set.star x"
-  thus "map f a \<in> Regular_Set.star (map f ` x)"
-    apply (induct a)
-    apply (simp add: Regular_Set.star_def)
-    apply (rule_tac x = 0 in exI, simp)
-    by (metis (lifting) append_in_starI image_eqI map_append star_if_lang)
-qed
-
-lemma image_star2: "Regular_Set.star (map f ` x) \<subseteq> map f ` Regular_Set.star x"
-proof auto
-  fix a assume "a \<in> Regular_Set.star (map f ` x)"
-  thus "a \<in> map f ` Regular_Set.star x"
-    apply (induct a)
-    apply auto
-    by (metis (lifting) append_in_starI image_iff map_append star_if_lang)
-qed
-
-lemma image_star: "map f ` Regular_Set.star x = Regular_Set.star (map f ` x)"
-  by (metis equalityI image_star1 image_star2)
-
-lemma change_atoms_map: shows "lang (change_atoms f \<alpha>) = lang_map f (lang \<alpha>)"
-  apply (induct \<alpha>)
-  apply (simp add: lang_map_def)
-  apply (simp add: lang_map_def)
-  apply (simp add: lang_map_def)
-  apply (simp add: lang_map_def)
-  apply (metis image_Un)
-  apply (simp add: lang_map_def)
-  apply (metis image_conc)
-  apply (simp add: lang_map_def)
-  by (metis image_star)
-
-lemma lang_change:
-  assumes bij_f: "bij f"
-  shows "lang (change_atoms f \<alpha>) = lang (change_atoms f \<beta>) \<Longrightarrow> lang \<alpha> = lang \<beta>"
-  by (insert bij_lang_map[OF bij_f], simp add: change_atoms_map bij_def inj_on_def)
-
-theorem changed_soundness:
-  assumes bij_f: "bij f"
-  shows "check_eqv (change_atoms f \<alpha>) (change_atoms f \<beta>) \<Longrightarrow> lang \<alpha> = lang \<beta>"
-  by (metis soundness lang_change bij_f)
-
-(* FIXME: Construct correct bijection in tactic *)
-lemma bij_hack: "bij (\<lambda>x. 0::nat)" sorry
-
-context kleene_algebra
-begin
-
-  fun rexp_unfold :: "'a rexp \<Rightarrow> 'a" where
-    "rexp_unfold (Atom x) = x"
-  | "rexp_unfold (Plus x y) = rexp_unfold x + rexp_unfold y"
-  | "rexp_unfold (Times x y) = rexp_unfold x \<cdot> rexp_unfold y"
-  | "rexp_unfold One = 1"
-  | "rexp_unfold Zero = 0"
-  | "rexp_unfold (Star x) = (rexp_unfold x)\<^sup>\<star>"
-
-  lemma completeness:
-    assumes "rexp_unfold \<alpha> \<in> carrier A" and "rexp_unfold \<beta> \<in> carrier A"
-    shows "lang \<alpha> = lang \<beta> \<Longrightarrow> rexp_unfold \<alpha> = rexp_unfold \<beta>"
-    sorry
-
-end
-
-lemma ka_is_dioid: "kleene_algebra A \<Longrightarrow> dioid A"
-  by (simp add: kleene_algebra_def)
-
-lemma (in kleene_algebra) atoms_closed: "atoms \<alpha> \<subseteq> carrier A \<Longrightarrow> rexp_unfold \<alpha> \<in> carrier A"
-  by (induct \<alpha>, simp_all add: zero_closed one_closed add_closed mult_closed star_closed)
-
-fun mk_bij_fun :: "('a \<times> 'b) list \<times> 'b \<Rightarrow> 'a \<Rightarrow> 'b" where
-  "mk_bij_fun (((x, y)#xs), y') x' = (if x = x' then y else mk_bij_fun (xs, y') x')"
-| "mk_bij_fun ([], y') x' = y'"
+lemma (in kleene_algebra) ka_term_closure:
+  "ka_term_atoms x \<subseteq> carrier A \<Longrightarrow> ka_term_unfold x \<in> carrier A"
+  by (induct x, simp_all add: add_closed mult_closed one_closed zero_closed star_closed)
 
 ML {*
-fun safe_dest_comb ct = SOME (Thm.dest_comb ct)
-  handle CTERM _ => NONE
-
-datatype ctree = CNode of ctree * ctree
-               | CLeaf of cterm;
-
-fun mk_ctree ct =
-  case safe_dest_comb ct of
-    SOME (ct1, ct2) => CNode (mk_ctree ct1, mk_ctree ct2)
-  | NONE => CLeaf ct;
-
-fun flatten (CNode (t1, t2)) = flatten t1 @ flatten t2
-  | flatten (CLeaf c) = [c]
-
-fun delete_alpha_eq y (x::xs) =
-    if y aconvc x
-    then delete_alpha_eq y xs
-    else x :: (delete_alpha_eq y xs)
-  | delete_alpha_eq _ [] = []
-
-fun rem_alpha_eq (x::xs) = x :: rem_alpha_eq (delete_alpha_eq x xs)
-  | rem_alpha_eq [] = []
-
-val cvars = rem_alpha_eq o flatten o mk_ctree
-
-fun inst_thm thm ctrm = SOME (Drule.instantiate' [] [SOME ctrm] thm)
-  handle _ => NONE
-
-fun inst_thms thm ctrms = List.mapPartial (inst_thm thm) ctrms
-
-val dka_expand_vars_tac = Subgoal.FOCUS (fn {concl, context, ...} =>
-  let
-    val vars = cvars concl
-    val witnesses = Locale.get_witnesses context
-    val var_subst = hd (witnesses RL @{thms kleene_algebra.rexp_unfold.simps(1)[symmetric]})
-    val var_substs = inst_thms var_subst vars
-  in
-    Method.insert_tac var_substs 1 THEN REPEAT (etac @{thm ssubst} 1)
-  end)
-
+val ka_term_fold_tac =
+  term_fold_tac @{thm kleene_algebra.ka_term_fold_atom} @{thms kleene_algebra.ka_term_unfold.simps[symmetric]} @{thm kleene_algebra.ka_term_closure}
 *}
 
-method_setup ka = {*
+method_setup ka_closure = {*
 Scan.succeed (fn ctxt =>
   let
-    val (k::_) = Locale.get_witnesses ctxt
-    val vars = map fst (Variable.dest_fixes ctxt)
+    val witnesses = Locale.get_witnesses ctxt
+    val unfolds = witnesses RL @{thms kleene_algebra.ka_term_atoms.simps}
   in
-    METHOD (fn thms =>
-      dka_expand_vars_tac ctxt 1
-      THEN asm_full_simp_tac (HOL_basic_ss addsimps
-        (k :: @{thms ka_is_dioid dioid.nat_order_def kleene_algebra.rexp_unfold.simps[symmetric]})) 1
-      THEN rtac @{thm kleene_algebra.completeness} 1
-      THEN rtac k 1
-      THEN rtac @{thm kleene_algebra.atoms_closed} 1
-      THEN asm_full_simp_tac (HOL_basic_ss addsimps [k]) 1
-      THEN asm_full_simp_tac @{simpset} 1
-      THEN rtac @{thm kleene_algebra.atoms_closed} 1
-      THEN asm_full_simp_tac (HOL_basic_ss addsimps [k]) 1
-      THEN asm_full_simp_tac @{simpset} 1
-      THEN rtac @{thm changed_soundness[OF bij_hack]} 1
-      THEN asm_full_simp_tac @{simpset} 1
-      THEN eval_tac ctxt 1)
+    METHOD (fn _ =>
+      ka_term_fold_tac true ctxt 1
+      THEN asm_full_simp_tac (@{simpset} addsimps unfolds) 1)
   end)
 *}
 
 context kleene_algebra
 begin
 
-  lemma "x \<in> carrier A \<Longrightarrow> x\<^sup>\<star>\<cdot>x\<^sup>\<star> = x\<^sup>\<star>" by ka
+  lemma star_subdist:
+    assumes xc: "x \<in> carrier A" and yc: "y \<in> carrier A"
+    shows "x\<^sup>\<star> \<sqsubseteq> (x+y)\<^sup>\<star>"
+  proof -
+    have "x\<^sup>\<star>\<cdot>1 \<sqsubseteq> (x+y)\<^sup>\<star>"
+    proof (rule star_inductl[rule_format], insert xc yc, ka_closure+)
+      have "1 + x\<cdot>(x+y)\<^sup>\<star> \<sqsubseteq> 1 + (x+y)\<cdot>(x+y)\<^sup>\<star>"
+      proof (rule add_iso[rule_format, OF _ _ one_closed], insert xc yc, ka_closure+)
+        show "x\<cdot>(x+y)\<^sup>\<star> \<sqsubseteq> (x+y)\<cdot>(x+y)\<^sup>\<star>"
+          by (metis add_closed add_lub mult_isor nat_refl star_closed xc yc)
+      qed
+      moreover have "... \<sqsubseteq> (x+y)\<^sup>\<star>"
+        by (metis add_closed star_unfoldl xc yc)
+      ultimately show "1 + x\<cdot>(x+y)\<^sup>\<star> \<sqsubseteq> (x+y)\<^sup>\<star>"
+        by (rule nat_trans, insert xc yc, ka_closure+)
+    qed
+    thus ?thesis
+      by (metis mult_oner star_closed xc)
+  qed
 
-  lemma "x \<in> carrier A \<Longrightarrow> x + x \<sqsubseteq> x\<^sup>\<star>" by ka
+  lemma star_iso: "\<lbrakk>x \<in> carrier A; y \<in> carrier A\<rbrakk> \<Longrightarrow> x \<sqsubseteq> y \<longrightarrow> x\<^sup>\<star> \<sqsubseteq> y\<^sup>\<star>"
+    by (metis nat_order_def star_subdist)
+
+  lemma star_ext: "x \<in> carrier A \<Longrightarrow> x \<sqsubseteq> x\<^sup>\<star>"
+    by (smt mult_closed mult_oner nat_trans one_closed star_1l star_closed star_plus_one subdistl)
+
+  lemma add_lub_r1:
+    "\<lbrakk>x \<in> carrier A; y \<in> carrier A; z \<in> carrier A; x \<sqsubseteq> z; y \<sqsubseteq> z\<rbrakk> \<Longrightarrow> x + y \<sqsubseteq> z"
+    by (metis add_lub)
+
+  lemma star_sim1:
+    assumes xc: "x \<in> carrier A" and yc: "y \<in> carrier A" and zc: "z \<in> carrier A"
+    shows "x\<cdot>z \<sqsubseteq> z\<cdot>y \<longrightarrow> x\<^sup>\<star>\<cdot>z \<sqsubseteq> z\<cdot>y\<^sup>\<star>"
+  proof
+    assume asm: "x\<cdot>z \<sqsubseteq> z\<cdot>y"
+    show "x\<^sup>\<star> \<cdot> z \<sqsubseteq> z \<cdot> y\<^sup>\<star>"
+    proof (rule star_inductl[rule_format], insert xc yc zc, ka_closure+)
+      show "z + x \<cdot> (z \<cdot> y\<^sup>\<star>) \<sqsubseteq> z \<cdot> y\<^sup>\<star>"
+      proof (rule add_lub_r1, insert xc yc zc, ka_closure+)
+        show "z \<sqsubseteq> z\<cdot>y\<^sup>\<star>"
+          by (smt mult_double_iso mult_oner nat_refl one_closed star_closed star_ref yc zc)
+        have "x\<cdot>(z\<cdot>y\<^sup>\<star>) = x\<cdot>z\<cdot>y\<^sup>\<star>"
+          by (metis mult_assoc star_closed xc yc zc)
+        moreover have "... \<sqsubseteq> z\<cdot>y\<cdot>y\<^sup>\<star>"
+          by (metis asm mult_closed mult_isor star_closed xc yc zc)
+        moreover have "... \<sqsubseteq> z\<cdot>(y\<cdot>y\<^sup>\<star>)"
+          by (metis mult_assoc mult_closed nat_refl star_closed yc zc)
+        moreover have "... \<sqsubseteq> z\<cdot>y\<^sup>\<star>"
+          by (metis mult_closed mult_isol star_1l star_closed yc zc)
+        ultimately show "x\<cdot>(z\<cdot>y\<^sup>\<star>) \<sqsubseteq> z\<cdot>y\<^sup>\<star>"
+          by (smt mult_closed nat_trans star_closed xc yc zc)
+      qed
+    qed
+  qed
+
+  lemma star_slide1: "\<lbrakk>x \<in> carrier A; y \<in> carrier A\<rbrakk> \<Longrightarrow> (x\<cdot>y)\<^sup>\<star>\<cdot>x \<sqsubseteq> x\<cdot>(y\<cdot>x)\<^sup>\<star>"
+    by (metis mult_assoc mult_closed nat_refl star_sim1)
+
+  lemma star_slide_var1: "x \<in> carrier A \<Longrightarrow> x\<^sup>\<star>\<cdot>x \<sqsubseteq> x\<cdot>x\<^sup>\<star>"
+    by (frule star_slide1[OF _ one_closed], metis mult_onel mult_oner)
+
+  lemma star2: assumes xc: "x \<in> carrier A" shows "(1+x)\<^sup>\<star> = x\<^sup>\<star>"
+  proof -
+    have "x\<^sup>\<star> \<sqsubseteq> (1+x)\<^sup>\<star>"
+      by (metis add_comm assms one_closed star_subdist)
+    moreover have "(1+x)\<^sup>\<star> \<sqsubseteq> x\<^sup>\<star>"
+      by (metis add_closed add_lub assms mult_oner one_closed star_closed star_ext star_invol star_iso star_ref)
+    ultimately show ?thesis
+      by (metis add_closed assms nat_antisym one_closed star_closed)
+  qed
+
+  lemma star_unfoldl_eq: assumes xc: "x \<in> carrier A" shows "x\<^sup>\<star> = 1+x\<cdot>x\<^sup>\<star>"
+  proof -
+    have "x\<^sup>\<star>\<cdot>1 \<sqsubseteq> 1 + x\<cdot>x\<^sup>\<star>"
+    proof (rule star_inductl[rule_format], insert xc, ka_closure+)
+      show "1 + x \<cdot> (1 + x \<cdot> x\<^sup>\<star>) \<sqsubseteq> 1 + x \<cdot> x\<^sup>\<star>"
+        apply (rule add_iso[rule_format], insert xc, ka_closure+)
+        apply (rule mult_isol[rule_format], ka_closure+)
+        by (rule star_unfoldl)
+    qed
+    thus ?thesis
+      by (metis xc add_closed mult_closed mult_oner nat_antisym one_closed star_closed star_unfoldl)
+  qed
+
+  lemma star_rtc1: "x \<in> carrier A \<Longrightarrow> 1+x+x\<^sup>\<star>\<cdot>x\<^sup>\<star> \<sqsubseteq> x\<^sup>\<star>"
+    by (metis add_assoc nat_order_def one_closed star_closed star_ext star_plus_one star_trans star_trans_eq)
+
+  lemma star_slide: assumes xc: "x \<in> carrier A" and yc: "y \<in> carrier A"
+    shows "(x\<cdot>y)\<^sup>\<star>\<cdot>x = x\<cdot>(y\<cdot>x)\<^sup>\<star>"
+  proof -
+    have "x\<cdot>(y\<cdot>x)\<^sup>\<star> \<sqsubseteq> (x\<cdot>y)\<^sup>\<star>\<cdot>x"
+      apply (rule star_inductr[rule_format], insert xc yc, ka_closure+)
+      apply (rule add_lub_r1, ka_closure+)
+      apply (smt mult_closed mult_double_iso mult_onel nat_refl one_closed star_closed star_ref)
+      by (metis mult_assoc mult_closed mult_isol mult_isor star_closed star_ext star_trans_eq)
+    thus ?thesis
+      by (metis mult_closed nat_antisym star_closed star_slide1 xc yc)
+  qed
 
 end
 
